formal/fstar/ocaml-output/RDF_Entailment_Regime.ml
@@ -6,22 +6,114 @@ let rdf_reifies_iri : RDF_Term.wf_iri=
 let rdfs_proposition_iri : RDF_Term.wf_iri=
   "http://www.w3.org/2000/01/rdf-schema#Proposition"
 let owl_sameas_iri : RDF_Term.wf_iri= "http://www.w3.org/2002/07/owl#sameAs"
+let rdf_json_iri : RDF_Term.wf_iri=
+  "http://www.w3.org/1999/02/22-rdf-syntax-ns#JSON"
+let rec json_value_eq (fuel : Prims.nat) (v1 : Parser_JSON.json_val)
+  (v2 : Parser_JSON.json_val) : Prims.bool=
+  if fuel = Prims.int_zero
+  then false
+  else
+    (match (v1, v2) with
+     | (Parser_JSON.JNull, Parser_JSON.JNull) -> true
+     | (Parser_JSON.JBool a, Parser_JSON.JBool b) -> a = b
+     | (Parser_JSON.JString a, Parser_JSON.JString b) -> a = b
+     | (Parser_JSON.JNumber a, Parser_JSON.JNumber b) ->
+         XSD_IEEE754.json_number_eq a b
+     | (Parser_JSON.JArray xs, Parser_JSON.JArray ys) ->
+         json_arr_eq (fuel - Prims.int_one) xs ys
+     | (Parser_JSON.JObject fs, Parser_JSON.JObject gs) ->
+         ((FStar_List_Tot_Base.length fs) = (FStar_List_Tot_Base.length gs))
+           && (json_obj_eq (fuel - Prims.int_one) fs gs)
+     | (uu___1, uu___2) -> false)
+and json_arr_eq (fuel : Prims.nat) (xs : Parser_JSON.json_val Prims.list)
+  (ys : Parser_JSON.json_val Prims.list) : Prims.bool=
+  if fuel = Prims.int_zero
+  then false
+  else
+    (match (xs, ys) with
+     | ([], []) -> true
+     | (x::xr, y::yr) ->
+         (json_value_eq (fuel - Prims.int_one) x y) &&
+           (json_arr_eq (fuel - Prims.int_one) xr yr)
+     | (uu___1, uu___2) -> false)
+and json_obj_eq (fuel : Prims.nat)
+  (fs : (Prims.string * Parser_JSON.json_val) Prims.list)
+  (gs : (Prims.string * Parser_JSON.json_val) Prims.list) : Prims.bool=
+  if fuel = Prims.int_zero
+  then false
+  else
+    (match fs with
+     | [] -> true
+     | (k, v)::rest ->
+         (match FStar_List_Tot_Base.assoc k gs with
+          | FStar_Pervasives_Native.Some v' ->
+              (json_value_eq (fuel - Prims.int_one) v v') &&
+                (json_obj_eq (fuel - Prims.int_one) rest gs)
+          | FStar_Pervasives_Native.None -> false))
+let rdf_json_value_eq (lex1 : Prims.string) (lex2 : Prims.string) :
+  Prims.bool=
+  match ((Parser_JSON.parse_json lex1), (Parser_JSON.parse_json lex2)) with
+  | (FStar_Pervasives_Native.Some v1, FStar_Pervasives_Native.Some v2) ->
+      json_value_eq
+        (((Parser_JSON.json_size v1) + (Parser_JSON.json_size v2)) +
+           Prims.int_one) v1 v2
+  | (uu___, uu___1) -> lex1 = lex2
 let is_exact_scaled_dt (dt : RDF_Term.wf_iri) : Prims.bool=
   (dt = RDF_Term.xsd_integer) || (dt = RDF_Term.xsd_decimal)
-let dt_value_leq (l1 : RDF_Term.literal) (l2 : RDF_Term.literal) :
+let lit_opaque_eq (l1 : RDF_Term.literal) (l2 : RDF_Term.literal) :
   Prims.bool=
+  (((l1.RDF_Term.lexical_form = l2.RDF_Term.lexical_form) &&
+      (l1.RDF_Term.datatype = l2.RDF_Term.datatype))
+     && (l1.RDF_Term.lang_tag = l2.RDF_Term.lang_tag))
+    && (l1.RDF_Term.direction = l2.RDF_Term.direction)
+let dt_value_leq (inside_tt : Prims.bool) (l1 : RDF_Term.literal)
+  (l2 : RDF_Term.literal) : Prims.bool=
   if
-    (is_exact_scaled_dt l1.RDF_Term.datatype) &&
-      (is_exact_scaled_dt l2.RDF_Term.datatype)
-  then
-    match ((XSD_Datatypes.literal_to_scaled l1),
-            (XSD_Datatypes.literal_to_scaled l2))
-    with
-    | (FStar_Pervasives_Native.Some s1, FStar_Pervasives_Native.Some s2) ->
-        (l1.RDF_Term.datatype = l2.RDF_Term.datatype) &&
-          ((XSD_Datatypes.scaled_cmp s1 s2) = Prims.int_zero)
-    | (uu___, uu___1) -> RDF_Term.literal_eq l1 l2
-  else RDF_Term.literal_eq l1 l2
+    (inside_tt &&
+       (FStar_Pervasives_Native.uu___is_Some l1.RDF_Term.direction))
+      && (FStar_Pervasives_Native.uu___is_Some l2.RDF_Term.direction)
+  then lit_opaque_eq l1 l2
+  else
+    if
+      (l1.RDF_Term.datatype = RDF_Term.xsd_double) &&
+        (l2.RDF_Term.datatype = RDF_Term.xsd_double)
+    then
+      XSD_IEEE754.double_value_eq l1.RDF_Term.lexical_form
+        l2.RDF_Term.lexical_form
+    else
+      if
+        (l1.RDF_Term.datatype = XSD_Datatypes.xsd_float) &&
+          (l2.RDF_Term.datatype = XSD_Datatypes.xsd_float)
+      then
+        XSD_IEEE754.float_value_eq l1.RDF_Term.lexical_form
+          l2.RDF_Term.lexical_form
+      else
+        if
+          (l1.RDF_Term.datatype = rdf_json_iri) &&
+            (l2.RDF_Term.datatype = rdf_json_iri)
+        then
+          rdf_json_value_eq l1.RDF_Term.lexical_form l2.RDF_Term.lexical_form
+        else
+          if
+            (is_exact_scaled_dt l1.RDF_Term.datatype) &&
+              (is_exact_scaled_dt l2.RDF_Term.datatype)
+          then
+            (match ((XSD_Datatypes.literal_to_scaled l1),
+                     (XSD_Datatypes.literal_to_scaled l2))
+             with
+             | (FStar_Pervasives_Native.Some s1, FStar_Pervasives_Native.Some
+                s2) ->
+                 (l1.RDF_Term.datatype = l2.RDF_Term.datatype) &&
+                   ((XSD_Datatypes.scaled_cmp s1 s2) = Prims.int_zero)
+             | (uu___4, uu___5) -> RDF_Term.literal_eq l1 l2)
+          else RDF_Term.literal_eq l1 l2
+let bnd_rdf (t : RDF_Term.rdf_term) : Prims.bool=
+  match t with
+  | RDF_Term.T_Literal l ->
+      Prims.op_Negation
+        (XSD_Datatypes.literal_ill_formed l.RDF_Term.datatype
+           l.RDF_Term.lexical_form)
+  | uu___ -> true
 let reifies_prop_triples (t : RDF_Triple.triple) :
   RDF_Triple.triple Prims.list=
   if t.RDF_Triple.p = rdf_reifies_iri
@@ -90,11 +182,11 @@ let owl_closure (ts : RDF_Triple.triple Prims.list) :
   FStar_List_Tot_Base.fold_left apply_sameas_pair ts (sameas_pairs ts)
 let entails_rdf (a : RDF_Triple.triple Prims.list)
   (b : RDF_Triple.triple Prims.list) : Prims.bool=
-  RDF_Entailment_Simple.entails_with dt_value_leq a b
+  RDF_Entailment_Simple.entails_with dt_value_leq bnd_rdf a b
 let entails_rdfs (a : RDF_Triple.triple Prims.list)
   (b : RDF_Triple.triple Prims.list) : Prims.bool=
-  RDF_Entailment_Simple.entails_with dt_value_leq (rdfs_closure a) b
+  RDF_Entailment_Simple.entails_with dt_value_leq bnd_rdf (rdfs_closure a) b
 let entails_rdfs_plus (a : RDF_Triple.triple Prims.list)
   (b : RDF_Triple.triple Prims.list) : Prims.bool=
-  RDF_Entailment_Simple.entails_with dt_value_leq
+  RDF_Entailment_Simple.entails_with dt_value_leq bnd_rdf
     (owl_closure (rdfs_closure a)) b
