formal/fstar/ocaml-output/RDF_Entailment_Simple.ml
@@ -22,7 +22,9 @@ let match_subj (b : binding) (ps : RDF_Term.subject) (gs : RDF_Term.subject)
            then FStar_Pervasives_Native.Some b
            else FStar_Pervasives_Native.None
        | RDF_Term.S_BNode uu___ -> FStar_Pervasives_Native.None)
-let rec match_term (leq : RDF_Term.literal -> RDF_Term.literal -> Prims.bool)
+let rec match_term
+  (leq : Prims.bool -> RDF_Term.literal -> RDF_Term.literal -> Prims.bool)
+  (bnd : RDF_Term.rdf_term -> Prims.bool) (inside_tt : Prims.bool)
   (b : binding) (pat : RDF_Term.rdf_term) (g : RDF_Term.rdf_term) :
   binding FStar_Pervasives_Native.option=
   match pat with
@@ -33,7 +35,9 @@ let rec match_term (leq : RDF_Term.literal -> RDF_Term.literal -> Prims.bool)
            then FStar_Pervasives_Native.Some b
            else FStar_Pervasives_Native.None
        | FStar_Pervasives_Native.None ->
-           FStar_Pervasives_Native.Some ((lbl, g) :: b))
+           if bnd g
+           then FStar_Pervasives_Native.Some ((lbl, g) :: b)
+           else FStar_Pervasives_Native.None)
   | RDF_Term.T_IRI i ->
       (match g with
        | RDF_Term.T_IRI j ->
@@ -44,7 +48,7 @@ let rec match_term (leq : RDF_Term.literal -> RDF_Term.literal -> Prims.bool)
   | RDF_Term.T_Literal l ->
       (match g with
        | RDF_Term.T_Literal m ->
-           if leq l m
+           if leq inside_tt l m
            then FStar_Pervasives_Native.Some b
            else FStar_Pervasives_Native.None
        | uu___ -> FStar_Pervasives_Native.None)
@@ -54,41 +58,48 @@ let rec match_term (leq : RDF_Term.literal -> RDF_Term.literal -> Prims.bool)
            if pp = gp
            then
              (match match_subj b ps gs with
-              | FStar_Pervasives_Native.Some b1 -> match_term leq b1 po go
+              | FStar_Pervasives_Native.Some b1 ->
+                  match_term leq bnd true b1 po go
               | FStar_Pervasives_Native.None -> FStar_Pervasives_Native.None)
            else FStar_Pervasives_Native.None
        | uu___ -> FStar_Pervasives_Native.None)
-let match_triple (leq : RDF_Term.literal -> RDF_Term.literal -> Prims.bool)
-  (b : binding) (tb : RDF_Triple.triple) (ta : RDF_Triple.triple) :
+let match_triple
+  (leq : Prims.bool -> RDF_Term.literal -> RDF_Term.literal -> Prims.bool)
+  (bnd : RDF_Term.rdf_term -> Prims.bool) (b : binding)
+  (tb : RDF_Triple.triple) (ta : RDF_Triple.triple) :
   binding FStar_Pervasives_Native.option=
   if tb.RDF_Triple.p = ta.RDF_Triple.p
   then
     match match_subj b tb.RDF_Triple.s ta.RDF_Triple.s with
     | FStar_Pervasives_Native.Some b1 ->
-        match_term leq b1 tb.RDF_Triple.o ta.RDF_Triple.o
+        match_term leq bnd false b1 tb.RDF_Triple.o ta.RDF_Triple.o
     | FStar_Pervasives_Native.None -> FStar_Pervasives_Native.None
   else FStar_Pervasives_Native.None
-let rec try_match (leq : RDF_Term.literal -> RDF_Term.literal -> Prims.bool)
-  (bs : RDF_Triple.triple Prims.list) (b : binding)
-  (a : RDF_Triple.triple Prims.list) : Prims.bool=
-  match bs with | [] -> true | tb::rest -> try_alts leq bs tb rest b a a
-and try_alts (leq : RDF_Term.literal -> RDF_Term.literal -> Prims.bool)
-  (bs : RDF_Triple.triple Prims.list) (tb : RDF_Triple.triple)
-  (rest : RDF_Triple.triple Prims.list) (b : binding)
-  (a : RDF_Triple.triple Prims.list) (cand : RDF_Triple.triple Prims.list) :
-  Prims.bool=
+let rec try_match
+  (leq : Prims.bool -> RDF_Term.literal -> RDF_Term.literal -> Prims.bool)
+  (bnd : RDF_Term.rdf_term -> Prims.bool) (bs : RDF_Triple.triple Prims.list)
+  (b : binding) (a : RDF_Triple.triple Prims.list) : Prims.bool=
+  match bs with | [] -> true | tb::rest -> try_alts leq bnd bs tb rest b a a
+and try_alts
+  (leq : Prims.bool -> RDF_Term.literal -> RDF_Term.literal -> Prims.bool)
+  (bnd : RDF_Term.rdf_term -> Prims.bool) (bs : RDF_Triple.triple Prims.list)
+  (tb : RDF_Triple.triple) (rest : RDF_Triple.triple Prims.list)
+  (b : binding) (a : RDF_Triple.triple Prims.list)
+  (cand : RDF_Triple.triple Prims.list) : Prims.bool=
   match cand with
   | [] -> false
   | ta::more ->
-      (match match_triple leq b tb ta with
+      (match match_triple leq bnd b tb ta with
        | FStar_Pervasives_Native.Some b1 ->
-           if try_match leq rest b1 a
+           if try_match leq bnd rest b1 a
            then true
-           else try_alts leq bs tb rest b a more
-       | FStar_Pervasives_Native.None -> try_alts leq bs tb rest b a more)
-let entails_with (leq : RDF_Term.literal -> RDF_Term.literal -> Prims.bool)
-  (a : RDF_Triple.triple Prims.list) (b : RDF_Triple.triple Prims.list) :
-  Prims.bool= try_match leq b [] a
+           else try_alts leq bnd bs tb rest b a more
+       | FStar_Pervasives_Native.None -> try_alts leq bnd bs tb rest b a more)
+let entails_with
+  (leq : Prims.bool -> RDF_Term.literal -> RDF_Term.literal -> Prims.bool)
+  (bnd : RDF_Term.rdf_term -> Prims.bool) (a : RDF_Triple.triple Prims.list)
+  (b : RDF_Triple.triple Prims.list) : Prims.bool= try_match leq bnd b [] a
 let simple_entails (a : RDF_Triple.triple Prims.list)
   (b : RDF_Triple.triple Prims.list) : Prims.bool=
-  entails_with RDF_Term.literal_eq a b
+  entails_with (fun uu___ l m -> RDF_Term.literal_eq l m) (fun uu___ -> true)
+    a b
